TermTests/DispatchAndFoldTest.lean
@@ -47,6 +47,17 @@ error: could not synthesize default value for parameter 'h' using tactics
 error: Tactic `decide` proved that the proposition
   (Head.lam.join Head.lam).isFunLike = false
 is false
+---
+error: could not synthesize default value for parameter 'hEta' using tactics
+---
+error: Tactic `decide` proved that the proposition
+  (Head.app (Head.var (Var.index DeBruijn.head)).isVar0).isEtaRedex
+      (Usage.scrutinize (Head.var (Var.index DeBruijn.head.tail))
+            (Usage.single DeBruijn.head.tail + (Usage.single DeBruijn.head).tail.many +
+              (Usage.single DeBruijn.head).tail.many) +
+          Usage.single DeBruijn.head).head =
+    false
+is false
 -/
 #guard_msgs (error) in
 def appFunBranches :=
@@ -59,7 +70,7 @@ def appFunBranches :=
 error: could not synthesize default value for parameter 'h' using tactics
 ---
 error: Tactic `decide` proved that the proposition
-  ((Head.ctorOf [Head.lit]).join Head.var).isCtorLike = false
+  ((Head.ctorOf [Head.lit]).join (Head.var (Var.index DeBruijn.head))).isCtorLike = false
 is false
 -/
 #guard_msgs (error) in
@@ -95,7 +106,7 @@ is false
 error: could not synthesize default value for parameter 'hStep' using tactics
 ---
 error: Tactic `decide` proved that the proposition
-  0 = 0 → Head.var ≠ Head.var
+  0 = 0 → (Head.var (Var.index DeBruijn.head)).isVar = false
 is false
 -/
 #guard_msgs (error) in
@@ -118,12 +129,14 @@ example : run appIfDef_term true 5 = 6 := rfl
 example : run appIfDef_term false 5 = 10 := rfl
 
 /--
-info: ((Term.var DeBruijnProj.head.tail).bool_casesOn
-      (Term.externCall (Spine.cons (Term.var DeBruijnProj.head) (Spine.cons (Term.nat_mk 1) Spine.nil))
-        (fun vs => LeanInitPureExtern.preludeExtern (PreludeExtern.lean_nat_add vs.1 vs.2.1)) appIfDef_term._proof_4 ⋯)
-      (Term.externCall (Spine.cons (Term.var DeBruijnProj.head) (Spine.cons (Term.nat_mk 2) Spine.nil))
-        (fun vs => LeanInitPureExtern.preludeExtern (PreludeExtern.lean_nat_mul vs.1 vs.2.1)) appIfDef_term._proof_4 ⋯)
-      appIfDef_term._proof_6 appIfDef_term._proof_7).lam.lam
+info: (((Term.var DeBruijnProj.head.tail).bool_casesOn
+          (Term.externCall (Spine.cons (Term.var DeBruijnProj.head) (Spine.cons (Term.nat_mk 1) Spine.nil))
+            (fun vs => LeanInitPureExtern.preludeExtern (PreludeExtern.lean_nat_add vs.1 vs.2.1)) ⋯ ⋯)
+          (Term.externCall (Spine.cons (Term.var DeBruijnProj.head) (Spine.cons (Term.nat_mk 2) Spine.nil))
+            (fun vs => LeanInitPureExtern.preludeExtern (PreludeExtern.lean_nat_mul vs.1 vs.2.1)) ⋯ ⋯)
+          ⋯ appIfDef_term._proof_7 appIfDef_term._proof_8 ⋯).lam
+      ⋯).lam
+  ⋯
 -/
 #guard_msgs in
 #reduce (proofs := false) (types := false) appIfDef_term
@@ -140,15 +153,16 @@ def appIfCompDef_term :=
 example : run appIfCompDef_term true 3 = 18 := rfl
 
 /--
-info: ((Term.externCall (Spine.cons (Term.var DeBruijnProj.head) (Spine.cons (Term.var DeBruijnProj.head) Spine.nil))
-          (fun vs => LeanInitPureExtern.preludeExtern (PreludeExtern.lean_nat_mul vs.1 vs.2.1))
-          appIfCompDef_term._proof_1 ⋯).letE
-      ((Term.var DeBruijnProj.head.tail.tail).bool_casesOn
-        (Term.externCall (Spine.cons (Term.var DeBruijnProj.head) (Spine.cons (Term.var DeBruijnProj.head) Spine.nil))
-          (fun vs => LeanInitPureExtern.preludeExtern (PreludeExtern.lean_nat_add vs.1 vs.2.1))
-          appIfCompDef_term._proof_1 ⋯)
-        (Term.nat_mk 0) appIfDef_term._proof_6 appIfCompDef_term._proof_4)
-      appIfCompDef_term._proof_5 ⋯ ⋯).lam.lam
+info: (((Term.externCall (Spine.cons (Term.var DeBruijnProj.head) (Spine.cons (Term.var DeBruijnProj.head) Spine.nil))
+              (fun vs => LeanInitPureExtern.preludeExtern (PreludeExtern.lean_nat_mul vs.1 vs.2.1)) ⋯ ⋯).letE
+          ((Term.var DeBruijnProj.head.tail.tail).bool_casesOn
+            (Term.externCall
+              (Spine.cons (Term.var DeBruijnProj.head) (Spine.cons (Term.var DeBruijnProj.head) Spine.nil))
+              (fun vs => LeanInitPureExtern.preludeExtern (PreludeExtern.lean_nat_add vs.1 vs.2.1)) ⋯ ⋯)
+            (Term.nat_mk 0) ⋯ appIfCompDef_term._proof_6 appIfCompDef_term._proof_7 ⋯)
+          appIfCompDef_term._proof_9 ⋯ ⋯).lam
+      ⋯).lam
+  ⋯
 -/
 #guard_msgs in
 #reduce (proofs := false) (types := false) appIfCompDef_term
@@ -162,9 +176,10 @@ def forceIfDef_term :=
     Term sig0 [] _ (TyWf.prim .bool ⇒ TyWf.thunk (TyWf.prim .nat) ⇒ TyWf.prim .nat) .lam)
 
 /--
-info: ((Term.var DeBruijnProj.head.tail).bool_casesOn (Term.nat_mk 5)
-      ((Term.var DeBruijnProj.head).thunk_force forceIfDef_term._proof_3 ⋯) appIfDef_term._proof_6
-      forceIfDef_term._proof_5).lam.lam
+info: (((Term.var DeBruijnProj.head.tail).bool_casesOn (Term.nat_mk 5) ((Term.var DeBruijnProj.head).thunk_force ⋯ ⋯) ⋯
+          forceIfDef_term._proof_6 forceIfDef_term._proof_7 ⋯).lam
+      ⋯).lam
+  ⋯
 -/
 #guard_msgs in
 #reduce (proofs := false) (types := false) forceIfDef_term
@@ -184,15 +199,16 @@ example : run appMatchDef_term ⟨⟨1, by decide⟩, (3, ())⟩ 4 = 7 := rfl
 example : run appMatchDef_term ⟨⟨0, by decide⟩, ()⟩ 4 = 4 := rfl
 
 /--
-info: ((Term.var DeBruijnProj.head.tail).taggedUnion_casesOn
-      (TaggedUnionCases.skip (Term.var DeBruijnProj.head)
-        (CtorsWithPayloadCases.here
-          (Term.externCall
-            (Spine.cons (Term.var DeBruijnProj.head.tail) (Spine.cons (Term.var DeBruijnProj.head) Spine.nil))
-            (fun vs => LeanInitPureExtern.preludeExtern (PreludeExtern.lean_nat_add vs.1 vs.2.1))
-            appIfCompDef_term._proof_1 ⋯)
-          TaggedUnionCasesRest.nil))
-      appMatchDef_term._proof_3 ⋯).lam.lam
+info: (((Term.var DeBruijnProj.head.tail).taggedUnion_casesOn
+          (TaggedUnionCases.skip (Term.var DeBruijnProj.head)
+            (CtorsWithPayloadCases.here
+              (Term.externCall
+                (Spine.cons (Term.var DeBruijnProj.head.tail) (Spine.cons (Term.var DeBruijnProj.head) Spine.nil))
+                (fun vs => LeanInitPureExtern.preludeExtern (PreludeExtern.lean_nat_add vs.1 vs.2.1)) ⋯ ⋯)
+              TaggedUnionCasesRest.nil))
+          ⋯ ⋯ ⋯).lam
+      ⋯).lam
+  ⋯
 -/
 #guard_msgs in
 #reduce (proofs := false) (types := false) appMatchDef_term
@@ -212,9 +228,10 @@ example : run foldNoAccDef_term 5 = 8 := rfl
 
 /--
 info: ((Term.var DeBruijnProj.head).nat_casesOn (Term.nat_mk 7)
-    (Term.externCall (Spine.cons (Term.var DeBruijnProj.head) (Spine.cons (Term.nat_mk 2) Spine.nil))
-      (fun vs => LeanInitPureExtern.preludeExtern (PreludeExtern.lean_nat_mul vs.1 vs.2.1)) appIfDef_term._proof_4 ⋯)
-    foldNoAccDef_term._proof_2).lam
+      (Term.externCall (Spine.cons (Term.var DeBruijnProj.head) (Spine.cons (Term.nat_mk 2) Spine.nil))
+        (fun vs => LeanInitPureExtern.preludeExtern (PreludeExtern.lean_nat_mul vs.1 vs.2.1)) ⋯ ⋯)
+      ⋯).lam
+  ⋯
 -/
 #guard_msgs in
 #reduce (proofs := false) (types := false) foldNoAccDef_term
@@ -235,11 +252,12 @@ example : run deepNoAcc_term 5 = 13 := rfl
 
 /--
 info: ((Term.var DeBruijnProj.head).nat_casesOn (Term.nat_mk 1)
-    ((Term.var DeBruijnProj.head).nat_casesOn (Term.nat_mk 2)
-      (Term.externCall (Spine.cons (Term.var DeBruijnProj.head) (Spine.cons (Term.nat_mk 10) Spine.nil))
-        (fun vs => LeanInitPureExtern.preludeExtern (PreludeExtern.lean_nat_add vs.1 vs.2.1)) appIfDef_term._proof_4 ⋯)
-      foldNoAccDef_term._proof_2)
-    foldNoAccDef_term._proof_2).lam
+      ((Term.var DeBruijnProj.head).nat_casesOn (Term.nat_mk 2)
+        (Term.externCall (Spine.cons (Term.var DeBruijnProj.head) (Spine.cons (Term.nat_mk 10) Spine.nil))
+          (fun vs => LeanInitPureExtern.preludeExtern (PreludeExtern.lean_nat_add vs.1 vs.2.1)) ⋯ ⋯)
+        ⋯)
+      ⋯).lam
+  ⋯
 -/
 #guard_msgs in
 #reduce (proofs := false) (types := false) deepNoAcc_term
@@ -263,11 +281,12 @@ example : run arrNoAcc_term #[1, 2, 3] = 3 := rfl
 
 /--
 info: ((Term.var DeBruijnProj.head).array_casesOn (Term.nat_mk 0)
-    ((Term.var DeBruijnProj.head.tail).array_casesOn (Term.var DeBruijnProj.head)
-      (Term.externCall (Spine.cons (Term.var DeBruijnProj.head.tail.tail) (Spine.cons (Term.nat_mk 3) Spine.nil))
-        (fun vs => LeanInitPureExtern.preludeExtern (PreludeExtern.lean_nat_mul vs.1 vs.2.1)) appIfDef_term._proof_4 ⋯)
-      arrNoAcc_term._proof_3 ⋯)
-    arrNoAcc_term._proof_3 ⋯).lam
+      ((Term.var DeBruijnProj.head.tail).array_casesOn (Term.var DeBruijnProj.head)
+        (Term.externCall (Spine.cons (Term.var DeBruijnProj.head.tail.tail) (Spine.cons (Term.nat_mk 3) Spine.nil))
+          (fun vs => LeanInitPureExtern.preludeExtern (PreludeExtern.lean_nat_mul vs.1 vs.2.1)) ⋯ ⋯)
+        ⋯ ⋯)
+      ⋯ ⋯).lam
+  ⋯
 -/
 #guard_msgs in
 #reduce (proofs := false) (types := false) arrNoAcc_term
